The new bigstep semantics is monotonic over store size

Semantic/FsubNext/Eval/BigStep.lean
@@ -4,6 +4,12 @@ import Semantic.FsubNext.Heap
 
 namespace FsubNext
 
+def pred_is_monotonic (pred : Heap -> Exp {} -> Prop) : Prop :=
+  ∀ {h1 h2 : Heap} {e},
+    h2.subsumes h1 ->
+    pred h1 e ->
+    pred h2 e
+
 inductive Eval : Heap -> Exp {} -> (Heap -> Exp {} -> Prop) -> Prop where
 | eval_val :
   (hv : Exp.IsVal v) ->
@@ -20,7 +26,8 @@ inductive Eval : Heap -> Exp {} -> (Heap -> Exp {} -> Prop) -> Prop where
   h x = some ⟨.tabs T0 e, hv⟩ ->
   Eval h (e.subst (Subst.openTVar .top)) Q ->
   Eval h (.tapp (.free x) S) Q
-| eval_letin {h : Heap} :
+| eval_letin {h : Heap} {Q1 : Heap -> Exp {} -> Prop} :
+  (hpred : pred_is_monotonic Q1) ->  -- this local Q1 must be monotonic
   Eval h e1 Q1 ->
   (h_val : ∀ {h1} {v : Exp {}},
     (hv : Exp.IsVal v) ->
@@ -34,5 +41,35 @@ inductive Eval : Heap -> Exp {} -> (Heap -> Exp {} -> Prop) -> Prop where
     Q1 h1 (.var x) ->
     Eval h1 (e2.subst (Subst.openVar x)) Q) ->
   Eval h (.letin e1 e2) Q
+
+theorem eval_monotonic {h1 h2 : Heap}
+  (hpred : pred_is_monotonic Q)
+  (hsub : h2.subsumes h1)
+  (heval : Eval h1 e Q) :
+  Eval h2 e Q := by
+  induction heval generalizing h2
+  case eval_val => grind [Eval, pred_is_monotonic]
+  case eval_var => grind [Eval, pred_is_monotonic]
+  case eval_apply hx _ ih =>
+    specialize ih hpred hsub
+    apply Eval.eval_apply
+    · apply hsub _ _ hx
+    · assumption
+  case eval_tapply hx _ ih =>
+    specialize ih hpred hsub
+    apply Eval.eval_tapply
+    · apply hsub _ _ hx
+    · assumption
+  case eval_letin Q1 hpred0 _ _ _ ih ih_val ih_var =>
+    specialize ih hpred0 hsub
+    apply Eval.eval_letin (Q1:=Q1) hpred0 ih
+    case h_val =>
+      intro h1 v hv hq1 l' hfresh
+      apply ih_val hv hq1 l' hfresh hpred
+      apply Heap.subsumes_refl
+    case h_var =>
+      intro h1 x hq1
+      apply ih_var hq1 hpred
+      apply Heap.subsumes_refl
 
 end FsubNext
